BoogieLang/Semantics.thy
@@ -6,7 +6,7 @@ begin
 
 subsection \<open>Values, State, Variable Context\<close>
 
-datatype ('k, 'p) L = MapVal "('k + 'p, ('k, 'p) L) map" |  MapKey "('k, 'k + 'p) map"
+datatype ('k, 'p) L = MapVal "('p, ('k, 'p) L) map" |  MapKey "('k, 'p) map"
 
 text \<open>The values (and as a result the semantics) are parametrized by the carrier type 'a for the 
 abstract values (values that have a type constructed via type constructors)
